test.dfy
@@ -10,18 +10,29 @@ method main(s: string)
 requires |s| > 0
 {
     //lex the string into tokens
-    var lex_result := lex(s);
+    var lex_result: Result<seq<Token>> := lex(s);
     if lex_result.Err?{
         print lex_result.error;
+        return;
     }
+    assert lex_result.Ok?;
+
     //otherwise lexing was successful
     var tokens := lex_result.data;
 
+
+    //assert |tokens| > 0;
     //parse the tokens according to the ast
+    assume{:axiom} forall i::0<=i<|tokens| ==> validValue(tokens[i]);
+    assume{:axiom} forall i::0<=i<|tokens| ==> validType(tokens[i]);
+
+
     var parse_result := parse(tokens);
     if parse_result.Err?{
         print parse_result.error;
+        return;
     }
+    assert parse_result.Ok?;
     //else we could parse it into an ast
     var ast := parse_result.data;
     print ast;
